vera/VerilogToSMT/VerilogToSMT.v
@@ -209,7 +209,7 @@ Section expr_to_smt.
   .
 
   Equations transfer_module_item : Verilog.module_item -> transf (SMTLib.term Sort_Bool) :=
-    transfer_module_item (Verilog.AlwaysComb (Verilog.BlockingAssign lhs rhs)) :=
+    transfer_module_item (Verilog.AlwaysComb (Verilog.BlockingAssign lhs _ rhs)) :=
       let* lhs_smt := assign_target_to_smt lhs in
       let* rhs_smt := expr_to_smt rhs in
       ret (SMTLib.Term_Eq lhs_smt rhs_smt);
